src/Analysis/Instances/Interval/Interval_DG.thy
@@ -62,21 +62,13 @@ text \<open>
 
 theorem ivl_dg_post_solution_collect_sound:
   assumes pp: "part_post_solution (ivl_dg_generator gs g bot0 s0d s0g) x sigma vars"
-    and cover_entry: "(cfg_entry g, ()) \<in> vars"
-    and cover_edge: "\<And>u a w. (u, a, w) \<in> intra g \<Longrightarrow> (w, ()) \<in> vars"
-    and cover_enter:
-      "\<And>c dst fs as p k. (c, CallEdge dst fs as, FunctionEntry p, k) \<in> calls g
-         \<Longrightarrow> (FunctionEntry p, ()) \<in> vars"
-    and cover_combine:
-      "\<And>c dst fs as p k. (c, CallEdge dst fs as, FunctionEntry p, k) \<in> calls g
-         \<Longrightarrow> (k, ()) \<in> vars"
+    and cover: "vars_cover g vars"
     and finI: "finite (intra g)"
     and finC: "finite (calls g)"
     and sound0: "S0 \<subseteq> \<lbrakk>s0d \<squnion> s0g\<rbrakk>"
   shows "ltr_collect gs g S0 v \<subseteq> ivl_dg_gamma sigma v"
   by (rule dg_post_solution_collect_sound_ltr_for
-        [OF pp cover_entry cover_edge cover_enter cover_combine
-            finI finC sound0[folded gamma_unit_def]])
+        [OF pp cover finI finC sound0[folded gamma_unit_def]])
 
 end
 
