src/CodegenCheck/Voblint_OCaml_Check.thy
@@ -21,7 +21,7 @@ text \<open>
 
 export_code
   analyse Sign_Analysis Interval_Analysis
-  imp_prog.make proc_decl_of
+  mk_program proc_decl_of
   SKIP com.Call Random com.If Assign Seq While Restore Unwind Return Check
   N V Plus Minus Times
   Bc bexp.Not And Or Less bexp.Eq
